Working through stack assembly

13StackAssembly/AssembleStack.thy
@@ -6,7 +6,7 @@ primrec assemble_stack_len :: "byte_code \<Rightarrow> nat" where
   "assemble_stack_len (BLookup x) = 1"
 | "assemble_stack_len (BPushCon k) = 6"
 | "assemble_stack_len (BPushLam pc) = 9"
-| "assemble_stack_len BApply = 1"
+| "assemble_stack_len BApply = 16"
 | "assemble_stack_len BReturn = 1"
 | "assemble_stack_len BJump = 1"
 
@@ -29,16 +29,28 @@ primrec assemble_stack_op :: "(nat \<Rightarrow> nat) \<Rightarrow> byte_code \<
     SAMov (Mem Stk),
     SAPush Vals Acc, 
     SAMov (Mem Hp)]"
-| "assemble_stack_op mp BApply = [undefined]"
+| "assemble_stack_op mp BApply = [
+    SAJump,
+    SAGet Hp,
+    SAAdd 1,
+    SAUnbackup,
+    SAPush Env Acc,
+    SAGet Hp,
+    SABackup,
+    SAAdd 1,
+    SAPop Vals,
+    SAPush Stk Acc,
+    SAMov (Mem Env),
+    SAPush Stk Acc,
+    SASub 13,
+    SAMov PC,
+    SAPush Env Acc,
+    SAPop Vals]"
 | "assemble_stack_op mp BReturn = [undefined]"
 | "assemble_stack_op mp BJump = [undefined]"
 
 (*   evu_lookup [simp]: "cd ! pc = BLookup x \<Longrightarrow> unstr_lookup e (sh (sp - 1)) x = Some y \<Longrightarrow>
     cd \<tturnstile> US h hp e ep vs vp sh sp (Suc pc) \<leadsto>\<^sub>u US h hp e ep (vs(vp := y)) (Suc vp) sh sp pc"
-| evu_apply [simp]: "cd ! pc = BApply \<Longrightarrow> h (vs vp) = Suc x \<Longrightarrow> 
-    cd \<tturnstile> US h hp e ep vs (Suc (Suc vp)) sh sp (Suc pc) \<leadsto>\<^sub>u 
-      US h hp (e(ep := vs (Suc vp), Suc ep := h (Suc (vs vp)))) (2 + ep) vs vp
-        (sh(sp := pc, Suc sp := Suc (Suc ep))) (2 + sp) (h (Suc (Suc (vs vp))))"
 | evu_return_normal [simp]: "cd ! pc = BReturn \<Longrightarrow> 
     cd \<tturnstile> US h hp e ep vs vp sh (Suc (Suc sp)) (Suc pc) \<leadsto>\<^sub>u US h hp e ep vs vp sh sp (sh sp)"
 | evu_return_end [simp]: "cd ! pc = BReturn \<Longrightarrow> 
@@ -59,34 +71,27 @@ fun assembly_map :: "byte_code list \<Rightarrow> nat \<Rightarrow> nat" where
 definition assemble_stack_code :: "byte_code list \<Rightarrow> sassm_code list" where
   "assemble_stack_code cd = concat (map (assemble_stack_op (assembly_map cd)) cd)"
 
+definition assemble_heap :: "(nat \<Rightarrow> nat) \<Rightarrow> (nat \<Rightarrow> nat) \<Rightarrow> nat \<Rightarrow> nat" where
+  "assemble_heap mp h x = (if x mod 3 = 2 \<and> h (x - 2) = 1 then mp (h x) else h x)"
+
+definition assemble_stack :: "(nat \<Rightarrow> nat) \<Rightarrow> (nat \<Rightarrow> nat) \<Rightarrow> nat \<Rightarrow> nat" where
+  "assemble_stack mp s x = (if even x then s x else mp (s x))"
+
 primrec assemble_state :: "(nat \<Rightarrow> nat) \<Rightarrow> unstr_state \<Rightarrow> sassm_state" where
   "assemble_state mp (US h hp e ep vs vp sh sp pc) = 
-    SAS (case_memory h e vs sh) (case_memory hp ep vp sp) 0 (mp pc)"
+    SAS (case_memory (assemble_heap mp h) e vs (assemble_stack mp sh)) 
+      (case_memory hp ep vp sp) 0 0 (mp pc)"
+
+abbreviation assm_state :: "byte_code list \<Rightarrow> unstr_state \<Rightarrow> sassm_state" where
+  "assm_state cd \<equiv> assemble_state (assembly_map cd)"
 
 lemma [simp]: "length (assemble_stack_op mp op) = assemble_stack_len op"
   by (induction op) simp_all
 
-theorem completesa [simp]: "
-  assemble_stack_code cd\<^sub>b \<tturnstile> assemble_state (assembly_map cd\<^sub>b) \<Sigma>\<^sub>u \<leadsto>\<^sub>s\<^sub>a \<Sigma>\<^sub>s\<^sub>a' \<Longrightarrow> 
-    \<exists>\<Sigma>\<^sub>s\<^sub>a'' \<Sigma>\<^sub>u'. iter (\<tturnstile> assemble_stack_code cd\<^sub>b \<leadsto>\<^sub>s\<^sub>a) \<Sigma>\<^sub>s\<^sub>a' (assemble_state (assembly_map cd\<^sub>b) \<Sigma>\<^sub>u') \<and> 
-      cd\<^sub>b \<tturnstile> \<Sigma>\<^sub>u \<leadsto>\<^sub>u \<Sigma>\<^sub>u'"
-proof (induction "assemble_stack_code cd\<^sub>b" "assemble_state (assembly_map cd\<^sub>b) \<Sigma>\<^sub>u" \<Sigma>\<^sub>s\<^sub>a' 
-       rule: evalsa.induct)
-  case (evsa_push pc m r mem ps acc)
-  thus ?case by simp
-next
-  case (evsa_pop pc m ps p mem acc)
-  thus ?case by simp
-next
-  case (evsa_mov pc m mem ps acc)
-  thus ?case by simp
-next
-  case (evsa_get pc m mem ps acc)
-  thus ?case by simp
-next
-  case (evsa_sub pc k mem ps acc)
-  thus ?case by simp
-qed
+theorem completesa [simp]: "assemble_stack_code cd\<^sub>b \<tturnstile>\<^sub>s\<^sub>a assm_state cd\<^sub>b \<Sigma>\<^sub>u = Some \<Sigma>\<^sub>s\<^sub>a' \<Longrightarrow> 
+  \<exists>n \<Sigma>\<^sub>s\<^sub>a'' \<Sigma>\<^sub>u'. iter_evalsa (assemble_stack_code cd\<^sub>b) n \<Sigma>\<^sub>s\<^sub>a' = Some (assm_state cd\<^sub>b \<Sigma>\<^sub>u') \<and> 
+    cd\<^sub>b \<tturnstile> \<Sigma>\<^sub>u \<leadsto>\<^sub>u \<Sigma>\<^sub>u'"
+  by simp
 
 lemma [simp]: "cd ! pc = op \<Longrightarrow> pc < length cd \<Longrightarrow> 
   assembly_map cd (Suc pc) = assemble_stack_len op + assembly_map cd pc"
@@ -130,77 +135,201 @@ lemma [simp]: "cd ! pc = op \<Longrightarrow> pc < length cd \<Longrightarrow> 0
 lemma [simp]: "m Hp = h \<Longrightarrow> m Env = e \<Longrightarrow> m Vals = vs \<Longrightarrow> m Stk = sh \<Longrightarrow> m = case_memory h e vs sh" 
   by rule (simp split: memory.splits)
 
+lemma assm_hp_lemma1: "3 dvd x \<Longrightarrow> assemble_heap mp h x = h x"
+  by (simp add: assemble_heap_def)
+
+lemma assm_hp_lemma2: "x mod 3 = 1 \<Longrightarrow> assemble_heap mp h x = h x"
+  by (simp add: assemble_heap_def)
+
+lemma assm_hp_lemma3: "x mod 3 = 2 \<Longrightarrow> h (x - 2) = 0 \<Longrightarrow> assemble_heap mp h x = h x"
+  by (simp add: assemble_heap_def)
+
+lemma assm_hp_lemma4: "x mod 3 = 2 \<Longrightarrow> h (x - 2) = 1 \<Longrightarrow> assemble_heap mp h x = mp (h x)"
+  by (simp add: assemble_heap_def)
+
+lemma assemble_heap_update_lemma [simp]: "3 dvd hp \<Longrightarrow> x \<noteq> hp \<Longrightarrow> x \<noteq> Suc hp \<Longrightarrow> 
+  x \<noteq> Suc (Suc hp) \<Longrightarrow> x mod 3 = 2 \<Longrightarrow> 
+    (h(hp := a, Suc hp := b, Suc (Suc hp) := c)) (x - 2) = h (x - 2)"
+proof (induction x)
+  case (Suc x)
+  from Suc(2, 3, 4, 5, 6) show ?case 
+  proof (induction x)
+    case (Suc x)
+    from Suc(6) have "3 dvd x" by presburger
+    with Suc(2, 3, 4, 5, 6) show ?case by auto
+  qed simp_all
+qed simp_all
+
+lemma [simp]: "3 dvd hp \<Longrightarrow> x \<noteq> hp \<Longrightarrow> x \<noteq> Suc hp \<Longrightarrow> x \<noteq> Suc (Suc hp) \<Longrightarrow> 
+  assemble_heap (assembly_map cd) (h(hp := a, Suc hp := b, Suc (Suc hp) := c)) x = 
+    assemble_heap (assembly_map cd) h x"
+proof (unfold assemble_heap_def, cases "x mod 3 = 2")
+  case True
+  assume "3 dvd hp" and "x \<noteq> hp" and "x \<noteq> Suc hp" and "x \<noteq> Suc (Suc hp)"
+  moreover with True have "(h(hp := a, Suc hp := b, Suc (Suc hp) := c)) (x - 2) = h (x - 2)" 
+    by (metis assemble_heap_update_lemma)
+  ultimately show "(if x mod 3 = 2 \<and> (h(hp := a, Suc hp := b, Suc (Suc hp) := c)) (x - 2) = 1
+    then assembly_map cd ((h(hp := a, Suc hp := b, Suc (Suc hp) := c)) x) 
+      else (h(hp := a, Suc hp := b, Suc (Suc hp) := c)) x) =
+        (if x mod 3 = 2 \<and> h (x - 2) = 1 then assembly_map cd (h x) else h x)" by simp
+next
+  case False
+  assume "x \<noteq> hp" and "x \<noteq> Suc hp" and "x \<noteq> Suc (Suc hp)"
+  hence "(x = hp \<longrightarrow> a = h hp) \<and> (x \<noteq> hp \<longrightarrow> (x = Suc hp \<longrightarrow> b = h (Suc hp)) \<and> 
+    (x \<noteq> Suc hp \<longrightarrow> x = Suc (Suc hp) \<longrightarrow> c = h (Suc (Suc hp))))" by simp
+  with False show "(if x mod 3 = 2 \<and> (h(hp := a, Suc hp := b, Suc (Suc hp) := c)) (x - 2) = 1
+    then assembly_map cd ((h(hp := a, Suc hp := b, Suc (Suc hp) := c)) x) 
+      else (h(hp := a, Suc hp := b, Suc (Suc hp) := c)) x) =
+        (if x mod 3 = 2 \<and> h (x - 2) = 1 then assembly_map cd (h x) else h x)" by simp
+qed
+
+lemma [simp]: "restructurable_heap h hp ep (length cd) \<Longrightarrow> 
+  (assemble_heap (assembly_map cd) h)(hp := 0, Suc hp := a, Suc (Suc hp) := b) = 
+    assemble_heap (assembly_map cd) (h(hp := 0, Suc hp := a, Suc (Suc hp) := b))"
+proof
+  fix x
+  let ?h = "h(hp := 0, Suc hp := a, Suc (Suc hp) := b)"
+  assume "restructurable_heap h hp ep (length cd)"
+  hence H: "3 dvd hp" by (simp add: restructurable_heap_def)
+  moreover hence "Suc hp mod 3 = 1" by presburger
+  moreover hence "Suc (Suc hp) mod 3 = 2" by presburger
+  ultimately show "
+    ((assemble_heap (assembly_map cd) h)(hp := 0, Suc hp := a, Suc (Suc hp) := b)) x =
+      assemble_heap (assembly_map cd) (h(hp := 0, Suc hp := a, Suc (Suc hp) := b)) x" 
+    by (simp add: assm_hp_lemma1 assm_hp_lemma2 assm_hp_lemma3)
+qed
+
+lemma [simp]: "restructurable_heap h hp ep (length cd) \<Longrightarrow> 
+  (assemble_heap (assembly_map cd) h)(hp := Suc 0, Suc hp := a, Suc (Suc hp) := assembly_map cd b) = 
+    assemble_heap (assembly_map cd) (h(hp := Suc 0, Suc hp := a, Suc (Suc hp) := b))"
+proof
+  fix x
+  let ?h = "h(hp := 0, Suc hp := a, Suc (Suc hp) := b)"
+  assume "restructurable_heap h hp ep (length cd)"
+  hence H: "3 dvd hp" by (simp add: restructurable_heap_def)
+  moreover hence "Suc hp mod 3 = 1" by presburger
+  moreover hence "Suc (Suc hp) mod 3 = 2" by presburger
+  ultimately show "((assemble_heap (assembly_map cd) h)(hp := Suc 0, Suc hp := a, 
+    Suc (Suc hp) := assembly_map cd b)) x =
+      assemble_heap (assembly_map cd) (h(hp := Suc 0, Suc hp := a, Suc (Suc hp) := b)) x" 
+    by (simp add: assm_hp_lemma1 assm_hp_lemma2 assm_hp_lemma4)
+qed
+
+lemma [simp]: "restructurable_vals vs (Suc (Suc vp)) hp \<Longrightarrow> 
+    assemble_heap mp h (Suc (vs vp)) = h (Suc (vs vp))"
+proof (unfold assemble_heap_def restructurable_vals_def)
+  assume "\<forall>x<Suc (Suc vp). 3 dvd vs x \<and> vs x < hp"
+  hence "3 dvd vs vp" by simp
+  hence "Suc (vs vp) mod 3 = 1" by presburger
+  thus "(if Suc (vs vp) mod 3 = 2 \<and> h (Suc (vs vp) - 2) = 1 then mp (h (Suc (vs vp))) 
+         else h (Suc (vs vp))) = h (Suc (vs vp))" by simp
+qed
+
+lemma [simp]: "h (vs vp) = Suc x \<Longrightarrow>
+    assemble_heap mp h (Suc (Suc (vs vp))) = h (Suc (Suc (vs vp)))"
+proof (unfold assemble_heap_def)
+  assume "h (vs vp) = Suc x"
+
+
+  show "(if Suc (Suc (vs vp)) mod 3 = 2 \<and> h (Suc (Suc (vs vp)) - 2) = 1 
+         then mp (h (Suc (Suc (vs vp)))) else h (Suc (Suc (vs vp)))) =
+    h (Suc (Suc (vs vp)))" by simp
+qed
+
+lemma [simp]: "odd sp \<Longrightarrow> assemble_stack (assembly_map cd) sh (sp - Suc 0) = sh (sp - Suc 0)"
+  by (simp add: assemble_stack_def)
+
+lemma [simp]: "odd sp \<Longrightarrow> 
+  ((assemble_stack (assembly_map cd) sh)(sp := assembly_map cd pc, Suc sp := a)) =
+    (assemble_stack (assembly_map cd) (sh(sp := pc, Suc sp := a)))"
+  by (auto simp add: assemble_stack_def)
+
 theorem correctsa [simp]: "cd\<^sub>b \<tturnstile> \<Sigma>\<^sub>u \<leadsto>\<^sub>u \<Sigma>\<^sub>u' \<Longrightarrow> restructurable \<Sigma>\<^sub>u cd\<^sub>b \<Longrightarrow> 
-  iter (\<tturnstile> assemble_stack_code cd\<^sub>b \<leadsto>\<^sub>s\<^sub>a) (assemble_state (assembly_map cd\<^sub>b) \<Sigma>\<^sub>u) 
-    (assemble_state (assembly_map cd\<^sub>b) \<Sigma>\<^sub>u')"
+  \<exists>n. iter_evalsa (assemble_stack_code cd\<^sub>b) n (assm_state cd\<^sub>b \<Sigma>\<^sub>u) = Some (assm_state cd\<^sub>b \<Sigma>\<^sub>u')"
 proof (induction cd\<^sub>b \<Sigma>\<^sub>u \<Sigma>\<^sub>u' rule: evalu.induct)
 case (evu_lookup cd pc x e sh sp y h hp ep vs vp)
   then show ?case by simp
 next
   case (evu_pushcon cd pc k h hp e ep vs vp sh sp)
-  let ?mem = "case_memory h e vs sh"
-  let ?ps = "case_memory hp ep vp sp"
-  from evu_pushcon have "assemble_stack_code cd ! (5 + assembly_map cd pc) = SAMov (Mem Hp)" by simp
-  hence "assemble_stack_code cd ! (Suc (Suc (Suc (Suc (Suc (assembly_map cd pc)))))) = 
-    SAMov (Mem Hp)" by (simp add: numeral_def)
-  hence A: "assemble_stack_code cd \<tturnstile> 
-    SAS ?mem ?ps 0 (Suc (Suc (Suc (Suc (Suc (Suc (assembly_map cd pc))))))) \<leadsto>\<^sub>s\<^sub>a 
-      SAS ?mem ?ps hp (Suc (Suc (Suc (Suc (Suc (assembly_map cd pc))))))" 
-    by (metis evsa_mov get_mval.simps(1) memory.simps(13))
-  from evu_pushcon have "assemble_stack_code cd ! (4 + assembly_map cd pc) = SAPush Vals Acc" 
-    by simp
-  hence "assemble_stack_code cd ! (Suc (Suc (Suc (Suc (assembly_map cd pc))))) = SAPush Vals Acc" 
-    by (simp add: numeral_def)
-  hence B: "
-    assemble_stack_code cd \<tturnstile> SAS ?mem ?ps hp (Suc (Suc (Suc (Suc (Suc (assembly_map cd pc)))))) \<leadsto>\<^sub>s\<^sub>a
-      SAS (mem_upd ?mem Vals vp hp) (?ps(Vals := Suc vp)) hp 
-        (Suc (Suc (Suc (Suc (assembly_map cd pc)))))"
-    by (metis evsa_push memory.simps(15) get_val.simps(1))
-  from evu_pushcon have "assemble_stack_code cd ! (3 + assembly_map cd pc) = SAPush Hp (Con 0)" 
-    by simp
-  hence "assemble_stack_code cd ! (Suc (Suc (Suc (assembly_map cd pc)))) = SAPush Hp (Con 0)" 
-    by (simp add: numeral_def)
-  hence C: "assemble_stack_code cd \<tturnstile> SAS (mem_upd ?mem Vals vp hp) (?ps(Vals := Suc vp)) hp 
-    (Suc (Suc (Suc (Suc (assembly_map cd pc))))) \<leadsto>\<^sub>s\<^sub>a SAS (mem_upd (mem_upd ?mem Vals vp hp) Hp hp 0) 
-      (?ps(Vals := Suc vp, Hp := Suc hp)) hp (Suc (Suc (Suc (assembly_map cd pc))))" 
-    by (metis evsa_push get_val.simps(2) fun_upd_apply memory.distinct(3) memory.simps(13))
-  from evu_pushcon have "assemble_stack_code cd ! (2 + assembly_map cd pc) = 
-    SAPush Hp (Con k)" by (simp del: add_2_eq_Suc)
-  hence "assemble_stack_code cd ! (Suc (Suc (assembly_map cd pc))) = SAPush Hp (Con k)" by simp
-  hence D: "assemble_stack_code cd \<tturnstile> SAS (mem_upd (mem_upd ?mem Vals vp hp) Hp hp 0) 
-    (?ps(Vals := Suc vp, Hp := Suc hp)) hp (Suc (Suc (Suc (assembly_map cd pc)))) \<leadsto>\<^sub>s\<^sub>a 
-      SAS (mem_upd (mem_upd (mem_upd ?mem Vals vp hp) Hp hp 0) Hp (Suc hp) k) 
-        (?ps(Vals := Suc vp, Hp := Suc (Suc hp))) hp (Suc (Suc (assembly_map cd pc)))" 
-    by (metis evsa_push get_val.simps(2) fun_upd_apply fun_upd_upd)
-  from evu_pushcon have "assemble_stack_code cd ! Suc (assembly_map cd pc) = SAPush Hp (Con 0)" 
-    by simp
-  hence E: "assemble_stack_code cd \<tturnstile> SAS (mem_upd (mem_upd (mem_upd ?mem Vals vp hp) Hp hp 0) Hp 
-    (Suc hp) k) (?ps(Vals := Suc vp, Hp := Suc (Suc hp))) hp (Suc (Suc (assembly_map cd pc))) \<leadsto>\<^sub>s\<^sub>a
-      SAS (mem_upd (mem_upd (mem_upd (mem_upd ?mem Vals vp hp) Hp hp 0) Hp (Suc hp) k) Hp 
-        (Suc (Suc hp)) 0) (?ps(Vals := Suc vp, Hp := Suc (Suc (Suc hp)))) hp 
-          (Suc (assembly_map cd pc))" 
-    by (metis evsa_push get_val.simps(2) fun_upd_apply fun_upd_upd)
-  from evu_pushcon have "assemble_stack_code cd ! assembly_map cd pc = SAMov (MCon 0)" by simp
-  hence "assemble_stack_code cd \<tturnstile> SAS 
-    (mem_upd (mem_upd (mem_upd (mem_upd ?mem Vals vp hp) Hp hp 0) Hp (Suc hp) k) Hp 
-      (Suc (Suc hp)) 0) (?ps(Vals := Suc vp, Hp := Suc (Suc (Suc hp)))) hp 
-        (Suc (assembly_map cd pc)) \<leadsto>\<^sub>s\<^sub>a SAS 
-          (mem_upd (mem_upd (mem_upd (mem_upd ?mem Vals vp hp) Hp hp 0) Hp (Suc hp) k) Hp 
-            (Suc (Suc hp)) 0) (?ps(Vals := Suc vp, Hp := Suc (Suc (Suc hp)))) 0 
-              (assembly_map cd pc)" 
-    by (metis evsa_mov get_mval.simps(2))
-  with A B C D E have "iter (\<tturnstile> assemble_stack_code cd \<leadsto>\<^sub>s\<^sub>a) 
-    (SAS ?mem ?ps 0 (Suc (Suc (Suc (Suc (Suc (Suc (assembly_map cd pc))))))))
-      (SAS (mem_upd (mem_upd (mem_upd (mem_upd ?mem Vals vp hp) Hp hp 0) Hp (Suc hp) k) Hp 
-        (Suc (Suc hp)) 0) (?ps(Vals := Suc vp, Hp := Suc (Suc (Suc hp)))) 0 (assembly_map cd pc))"
-    by simp
-  with evu_pushcon show ?case by (simp add: numeral_def)
+  moreover hence "assemble_stack_code cd ! (5 + assembly_map cd pc) = SAMov (Mem Hp)" by simp
+  moreover from evu_pushcon have "assemble_stack_code cd ! (4 + assembly_map cd pc) =
+    SAPush Vals Acc" by simp
+  moreover from evu_pushcon have "assemble_stack_code cd ! (3 + assembly_map cd pc) = 
+    SAPush Hp (Con 0)" by simp
+  moreover from evu_pushcon have "assemble_stack_code cd ! (2 + assembly_map cd pc) = 
+    SAPush Hp (Con k)" by (simp del: add_2_eq_Suc) 
+  ultimately have "iter_evalsa (assemble_stack_code cd) 6 (SAS (case_memory 
+    (assemble_heap (assembly_map cd) h) e vs (assemble_stack (assembly_map cd) sh)) 
+      (case_memory hp ep vp sp) 0 0 (assembly_map cd (Suc pc))) = 
+        Some (SAS (case_memory (assemble_heap (assembly_map cd) 
+          (h(hp := 0, Suc hp := k, Suc (Suc hp) := 0))) e (vs(vp := hp)) 
+            (assemble_stack (assembly_map cd) sh)) (case_memory (3 + hp) ep (Suc vp) sp) 0 0 
+              (assembly_map cd pc))" 
+    by (auto simp add: numeral_def)
+  thus ?case by auto
 next
   case (evu_pushlam cd pc pc' h hp e ep vs vp sh sp)
-  then show ?case by simp
+  moreover hence "assemble_stack_code cd ! (8 + assembly_map cd pc) = SAMov (Mem Hp)" by simp
+  moreover from evu_pushlam have "assemble_stack_code cd ! (7 + assembly_map cd pc) =
+    SAPush Vals Acc" by simp
+  moreover from evu_pushlam have "assemble_stack_code cd ! (6 + assembly_map cd pc) = 
+    SAMov (Mem Stk)" by simp
+  moreover from evu_pushlam have "assemble_stack_code cd ! (5 + assembly_map cd pc) = SASub 1" 
+    by simp
+  moreover from evu_pushlam have "assemble_stack_code cd ! (4 + assembly_map cd pc) = SAGet Stk" 
+    by simp
+  moreover from evu_pushlam have "assemble_stack_code cd ! (3 + assembly_map cd pc) = 
+    SAPush Hp (Con 1)" by simp 
+  moreover from evu_pushlam have "assemble_stack_code cd ! (2 + assembly_map cd pc) = 
+    SAPush Hp Acc" by (simp del: add_2_eq_Suc) 
+  ultimately have "iter_evalsa (assemble_stack_code cd) 9 (SAS (case_memory 
+    (assemble_heap (assembly_map cd) h) e vs (assemble_stack (assembly_map cd) sh)) 
+      (case_memory hp ep vp sp) 0 0 (assembly_map cd (Suc pc))) = Some (SAS (case_memory 
+        (assemble_heap (assembly_map cd) 
+          (h(hp := Suc 0, Suc hp := sh (sp - Suc 0), Suc (Suc hp) := pc'))) e (vs(vp := hp)) 
+            (assemble_stack (assembly_map cd) sh)) (case_memory (3 + hp) ep (Suc vp) sp) 0 0 
+              (assembly_map cd pc))" 
+    by (auto simp add: numeral_def)
+  thus ?case by auto
 next
   case (evu_apply cd pc h vs vp x hp e ep sh sp)
-  then show ?case by simp
+  moreover from evu_apply have "assemble_stack_code cd ! (15 + assembly_map cd pc) = SAPop Vals" 
+    by simp
+  moreover from evu_apply have "assemble_stack_code cd ! (14 + assembly_map cd pc) = SAPush Env Acc" 
+    by simp
+  moreover from evu_apply have "assemble_stack_code cd ! (13 + assembly_map cd pc) = SAMov PC" 
+    by simp
+  moreover from evu_apply have "assemble_stack_code cd ! (12 + assembly_map cd pc) = SASub 13" 
+    by simp
+  moreover from evu_apply have "assemble_stack_code cd ! (11 + assembly_map cd pc) = SAPush Stk Acc" 
+    by simp
+  moreover from evu_apply have "assemble_stack_code cd ! (10 + assembly_map cd pc) = 
+    SAMov (Mem Env)" by simp
+  moreover from evu_apply have "assemble_stack_code cd ! (9 + assembly_map cd pc) = SAPush Stk Acc" 
+    by simp
+  moreover from evu_apply have "assemble_stack_code cd ! (8 + assembly_map cd pc) = SAPop Vals" 
+    by simp
+  moreover from evu_apply have "assemble_stack_code cd ! (7 + assembly_map cd pc) = SAAdd 1" 
+    by simp
+  moreover from evu_apply have "assemble_stack_code cd ! (6 + assembly_map cd pc) = SABackup" 
+    by simp
+  moreover from evu_apply have "assemble_stack_code cd ! (5 + assembly_map cd pc) = SAGet Hp" 
+    by simp
+  moreover from evu_apply have "assemble_stack_code cd ! (4 + assembly_map cd pc) = SAPush Env Acc" 
+    by simp
+  moreover from evu_apply have "assemble_stack_code cd ! (3 + assembly_map cd pc) = SAUnbackup" 
+    by simp
+  moreover from evu_apply have "assemble_stack_code cd ! (2 + assembly_map cd pc) = SAAdd 1" 
+    by (simp del: add_2_eq_Suc)
+  ultimately have "iter_evalsa (assemble_stack_code cd) 16 (SAS (case_memory 
+    (assemble_heap (assembly_map cd) h) e vs (assemble_stack (assembly_map cd) sh)) 
+      (case_memory hp ep (Suc (Suc vp)) sp) 0 0 (assembly_map cd (Suc pc))) = 
+        Some (SAS (case_memory (assemble_heap (assembly_map cd) h) (e(ep := vs (Suc vp), 
+          Suc ep := h (Suc (vs vp)))) vs (assemble_stack (assembly_map cd) 
+            (sh(sp := pc, Suc sp := Suc (Suc ep))))) (case_memory hp (Suc (Suc ep)) vp 
+              (Suc (Suc sp))) 0 0 (assembly_map cd (h (Suc (Suc (vs vp))))))" 
+    by (auto simp add: numeral_def)
+  thus ?case by auto
 next
   case (evu_return_normal cd pc h hp e ep vs vp sh sp)
   then show ?case by simp
@@ -213,8 +342,22 @@ next
 qed
 
 theorem correctsa_iter [simp]: "iter (\<tturnstile> cd\<^sub>b \<leadsto>\<^sub>u) \<Sigma>\<^sub>u \<Sigma>\<^sub>u' \<Longrightarrow> restructurable \<Sigma>\<^sub>u cd\<^sub>b \<Longrightarrow> 
-  iter (\<tturnstile> assemble_stack_code cd\<^sub>b \<leadsto>\<^sub>s\<^sub>a) 
-    (assemble_state (assembly_map cd\<^sub>b) \<Sigma>\<^sub>u) (assemble_state (assembly_map cd\<^sub>b) \<Sigma>\<^sub>u')"
-  by (induction \<Sigma>\<^sub>u \<Sigma>\<^sub>u' rule: iter.induct) (force, metis correctsa iter_append preserve_restructure)
+  \<exists>n. iter_evalsa (assemble_stack_code cd\<^sub>b) n (assm_state cd\<^sub>b \<Sigma>\<^sub>u) = Some (assm_state cd\<^sub>b \<Sigma>\<^sub>u')"
+proof (induction \<Sigma>\<^sub>u \<Sigma>\<^sub>u' rule: iter.induct)
+  case (iter_refl \<Sigma>\<^sub>u)
+  have "iter_evalsa (assemble_stack_code cd\<^sub>b) 0 (assm_state cd\<^sub>b \<Sigma>\<^sub>u) = Some (assm_state cd\<^sub>b \<Sigma>\<^sub>u)" 
+    by simp
+  thus ?case by blast
+next
+  case (iter_step \<Sigma>\<^sub>u \<Sigma>\<^sub>u' \<Sigma>\<^sub>u'')
+  then obtain n where "iter_evalsa (assemble_stack_code cd\<^sub>b) n (assm_state cd\<^sub>b \<Sigma>\<^sub>u) = 
+    Some (assm_state cd\<^sub>b \<Sigma>\<^sub>u')" by fastforce
+  moreover from iter_step obtain m where "
+    iter_evalsa (assemble_stack_code cd\<^sub>b) m (assm_state cd\<^sub>b \<Sigma>\<^sub>u') = Some (assm_state cd\<^sub>b \<Sigma>\<^sub>u'')" 
+      by fastforce
+  ultimately have "iter_evalsa (assemble_stack_code cd\<^sub>b) (n + m) (assm_state cd\<^sub>b \<Sigma>\<^sub>u) = 
+    Some (assm_state cd\<^sub>b \<Sigma>\<^sub>u'')" by simp
+  thus ?case by blast
+qed
 
 end
