13StackAssembly/StackAssembly.thy
@@ -4,12 +4,11 @@ begin
 
 datatype memory = Hp | Env | Vals | Stk
 
-datatype pseudoreg = Acc | Con nat
-datatype pseudomem = Mem memory | MCon nat
+datatype pseudoreg = Acc | Acc2 | Con nat
+datatype pseudomem = Mem memory | PC | MCon nat
 
 datatype sassm_code = 
   BLookup nat
-  | BApply
   | BReturn
   | BJump
 
@@ -18,9 +17,13 @@ datatype sassm_code =
   | SAMov pseudomem
   | SAGet memory
   | SASub nat
+  | SAAdd nat
+  | SAJump
+  | SABackup
+  | SAUnbackup
 
 datatype sassm_state = 
-  SAS "memory \<Rightarrow> nat \<Rightarrow> nat" "memory \<Rightarrow> nat" nat nat
+  SAS "memory \<Rightarrow> nat \<Rightarrow> nat" "memory \<Rightarrow> nat" nat nat nat
 
 fun sassm_lookup :: "(nat \<Rightarrow> nat) \<Rightarrow> nat \<Rightarrow> nat \<rightharpoonup> nat" where
   "sassm_lookup h 0 x = None"
@@ -28,53 +31,38 @@ fun sassm_lookup :: "(nat \<Rightarrow> nat) \<Rightarrow> nat \<Rightarrow> nat
 | "sassm_lookup h (Suc (Suc p)) 0 = Some (h p)"
 | "sassm_lookup h (Suc (Suc p)) (Suc x) = sassm_lookup h (h (Suc p)) x"
 
-primrec get_val :: "pseudoreg \<Rightarrow> nat \<Rightarrow> nat" where
-  "get_val Acc x = x"
-| "get_val (Con k) x = k"
+primrec get_val :: "pseudoreg \<Rightarrow> nat \<Rightarrow> nat \<Rightarrow> nat" where
+  "get_val Acc x y = x"
+| "get_val Acc2 x y = y"
+| "get_val (Con k) x y = k"
 
-primrec get_mval :: "pseudomem \<Rightarrow> (memory \<Rightarrow> nat) \<Rightarrow> nat" where
-  "get_mval (Mem m) x = x m"
-| "get_mval (MCon k) x = k"
+primrec get_mval :: "pseudomem \<Rightarrow> (memory \<Rightarrow> nat) \<Rightarrow> nat \<Rightarrow> nat" where
+  "get_mval (Mem m) x y = x m"
+| "get_mval PC x y = y"
+| "get_mval (MCon k) x y = k"
 
 fun mem_upd :: "(memory \<Rightarrow> nat \<Rightarrow> nat) \<Rightarrow> memory \<Rightarrow> nat \<Rightarrow> nat \<Rightarrow> memory \<Rightarrow> nat \<Rightarrow> nat" where
   "mem_upd mem m mp k m' x = (if m = m' \<and> mp = x then k else mem m' x)"
 
-inductive evalsa :: "sassm_code list \<Rightarrow> sassm_state \<Rightarrow> sassm_state \<Rightarrow> bool" 
-    (infix "\<tturnstile> _ \<leadsto>\<^sub>s\<^sub>a" 50) where
-  evsa_push [simp]: "cd ! pc = SAPush m r \<Longrightarrow>
-    cd \<tturnstile> SAS mem ps acc (Suc pc) \<leadsto>\<^sub>s\<^sub>a
-      SAS (mem_upd mem m (ps m) (get_val r acc)) (ps(m := Suc (ps m))) acc pc"
-| evsa_pop [simp]: "cd ! pc = SAPop m \<Longrightarrow> ps m = Suc p \<Longrightarrow>
-    cd \<tturnstile> SAS mem ps acc (Suc pc) \<leadsto>\<^sub>s\<^sub>a SAS mem (ps(m := p)) (mem m p) pc"
-| evsa_mov [simp]: "cd ! pc = SAMov m \<Longrightarrow>
-    cd \<tturnstile> SAS mem ps acc (Suc pc) \<leadsto>\<^sub>s\<^sub>a SAS mem ps (get_mval m ps) pc"
-| evsa_get [simp]: "cd ! pc = SAGet m \<Longrightarrow>
-    cd \<tturnstile> SAS mem ps acc (Suc pc) \<leadsto>\<^sub>s\<^sub>a SAS mem ps (mem m acc) pc"
-| evsa_sub [simp]: "cd ! pc = SASub k \<Longrightarrow>
-    cd \<tturnstile> SAS mem ps acc (Suc pc) \<leadsto>\<^sub>s\<^sub>a SAS mem ps (acc - k) pc"
+fun evalsa :: "sassm_code list \<Rightarrow> sassm_state \<rightharpoonup> sassm_state" (infix "\<tturnstile>\<^sub>s\<^sub>a" 50) where
+  "cd \<tturnstile>\<^sub>s\<^sub>a SAS mem ps acc acc2 0 = None"
+| "cd \<tturnstile>\<^sub>s\<^sub>a SAS mem ps acc acc2 (Suc pc) = (case cd ! pc of
+      SAPush m r \<Rightarrow> 
+        Some (SAS (mem_upd mem m (ps m) (get_val r acc pc)) (ps(m := Suc (ps m))) acc acc2 pc)
+    | SAPop m \<Rightarrow> (case ps m of
+          Suc p \<Rightarrow> Some (SAS mem (ps(m := p)) (mem m p) acc2 pc)
+        | 0 \<Rightarrow> None)
+    | SAMov m \<Rightarrow> Some (SAS mem ps (get_mval m ps pc) acc2 pc)
+    | SAGet m \<Rightarrow> Some (SAS mem ps (mem m acc) acc2 pc)
+    | SASub k \<Rightarrow> Some (SAS mem ps (acc - k) acc2 pc)
+    | SAAdd k \<Rightarrow> Some (SAS mem ps (acc + k) acc2 pc)
+    | SAJump \<Rightarrow> Some (SAS mem ps 0 0 acc)
+    | SABackup \<Rightarrow> Some (SAS mem ps acc acc pc)
+    | SAUnbackup \<Rightarrow> Some (SAS mem ps acc2 acc2 pc))"
 
-theorem determinismu: "cd \<tturnstile> \<Sigma> \<leadsto>\<^sub>s\<^sub>a \<Sigma>' \<Longrightarrow> cd \<tturnstile> \<Sigma> \<leadsto>\<^sub>s\<^sub>a \<Sigma>'' \<Longrightarrow> \<Sigma>' = \<Sigma>''"
-proof (induction cd \<Sigma> \<Sigma>' rule: evalsa.induct)
-  case (evsa_push cd pc m r mem ps acc)
-  from evsa_push(2, 1) show ?case 
-    by (induction cd "SAS mem ps acc (Suc pc)" \<Sigma>'' rule: evalsa.induct) simp_all
-next
-  case (evsa_pop cd pc m ps p mem acc)
-  from evsa_pop(3, 1, 2) show ?case 
-    by (induction cd "SAS mem ps acc (Suc pc)" \<Sigma>'' rule: evalsa.induct) simp_all
-next
-  case (evsa_mov cd pc m mem ps acc)
-  from evsa_mov(2, 1) show ?case 
-    by (induction cd "SAS mem ps acc (Suc pc)" \<Sigma>'' rule: evalsa.induct) simp_all
-next
-  case (evsa_get cd pc m mem ps acc)
-  from evsa_get(2, 1) show ?case 
-    by (induction cd "SAS mem ps acc (Suc pc)" \<Sigma>'' rule: evalsa.induct) simp_all
-next
-  case (evsa_sub cd pc k mem ps acc)
-  from evsa_sub(2, 1) show ?case 
-    by (induction cd "SAS mem ps acc (Suc pc)" \<Sigma>'' rule: evalsa.induct) simp_all
-qed
+primrec iter_evalsa :: "sassm_code list \<Rightarrow> nat \<Rightarrow> sassm_state \<rightharpoonup> sassm_state" where
+  "iter_evalsa cd 0 \<Sigma> = Some \<Sigma>"
+| "iter_evalsa cd (Suc x) \<Sigma> = Option.bind (cd \<tturnstile>\<^sub>s\<^sub>a \<Sigma>) (iter_evalsa cd x)"
 
 lemma [simp]: "mem_upd (case_memory h e vs sh) Hp x y = case_memory (h(x := y)) e vs sh"
   by (rule+) (simp split: memory.splits)
@@ -99,5 +87,12 @@ lemma [simp]: "(case_memory hp ep vp sp)(Vals := x) = case_memory hp ep x sp"
 
 lemma [simp]: "(case_memory hp ep vp sp)(Stk := x) = case_memory hp ep vp x"
   by rule (simp split: memory.splits)
+
+lemma [simp]: "iter_evalsa cd n \<Sigma> = Some \<Sigma>' \<Longrightarrow> iter_evalsa cd m \<Sigma>' = Some \<Sigma>'' \<Longrightarrow> 
+  iter_evalsa cd (n + m) \<Sigma> = Some \<Sigma>''"
+proof (induction n arbitrary: \<Sigma>)
+  case (Suc n)
+  then show ?case by (cases "cd \<tturnstile>\<^sub>s\<^sub>a \<Sigma>") simp_all
+qed simp_all
 
 end
